Adding Nondeterminism to binencoder specs.

src/BinEncoders/Env/Lib2/AsciiOpt.v
@@ -14,8 +14,13 @@ Section Ascii.
   Context {transformer : Transformer B}.
   Context {transformerUnit : TransformerUnitOpt transformer bool}.
 
-  Definition encode_ascii (c : ascii) (ce : CacheEncode) : B * CacheEncode :=
-    encode_word (NToWord 8 (N_of_ascii c)) ce.
+  Definition encode_ascii_Spec (c : ascii) (ce : CacheEncode)
+    : Comp (B * CacheEncode) :=
+    encode_word_Spec (NToWord 8 (N_of_ascii c)) ce.
+
+  Definition encode_ascii_Impl (c : ascii) (ce : CacheEncode)
+    : B * CacheEncode :=
+    encode_word_Impl (NToWord 8 (N_of_ascii c)) ce.
 
   Definition decode_ascii (b : B) (cd : CacheDecode) : option (ascii * B * CacheDecode) :=
     `(n, b, cd) <- decode_word (sz:=8) b cd;
@@ -23,30 +28,52 @@ Section Ascii.
 
   Open Local Scope nat.
   Theorem Ascii_decode_correct :
-    encode_decode_correct_f cache transformer (fun n => True) encode_ascii decode_ascii.
+    encode_decode_correct_f cache transformer (fun n => True) encode_ascii_Spec decode_ascii.
   Proof.
-    unfold encode_decode_correct, encode_ascii, decode_ascii.
-    intros env env' xenv c c' ext Eeq Ppred Penc.
-    destruct (Word_decode_correct _ _ _ _ _ ext Eeq I Penc) as [? [? ?] ].
-    rewrite H; simpl.
-    eexists; intuition eauto.
-    repeat f_equal.
-    rewrite wordToN_nat. rewrite NToWord_nat.
-    destruct (wordToNat_natToWord' 8 (BinNat.N.to_nat (N_of_ascii c))).
-    assert (x0 = 0).
-    { destruct x0; eauto; exfalso.
-      remember (wordToNat (natToWord 8 (BinNat.N.to_nat (N_of_ascii c)))) as xx; clear Heqxx.
-      replace (xx + S x0 * pow2 8) with (256 + (xx + x0 * 256)) in H1.
-      assert (BinNat.N.to_nat (N_of_ascii c) < 256).
-      assert (N.lt (N_of_ascii c) 256).
-      clear H. induction c; repeat (match goal with
-                                    | B : bool |- _ => destruct B
-                                    end); simpl; unfold Nlt; eauto.
-      change (256%nat) with (N.to_nat 256).
-      apply Nomega.Nlt_out. eauto.
-      omega. change (pow2 8) with 256. omega.
+    unfold decode_ascii; split.
+    { 
+      intros env env' xenv c c' ext Eeq Ppred Penc.
+      destruct (proj1 Word_decode_correct _ _ _ _ _ ext Eeq I Penc) as [? [? ?] ].
+      rewrite H; simpl.
+      eexists; intuition eauto.
+      repeat f_equal.
+      rewrite wordToN_nat. rewrite NToWord_nat.
+      destruct (wordToNat_natToWord' 8 (BinNat.N.to_nat (N_of_ascii c))).
+      assert (x0 = 0).
+      { destruct x0; eauto; exfalso.
+        remember (wordToNat (natToWord 8 (BinNat.N.to_nat (N_of_ascii c)))) as xx; clear Heqxx.
+        replace (xx + S x0 * pow2 8) with (256 + (xx + x0 * 256)) in H1.
+        assert (BinNat.N.to_nat (N_of_ascii c) < 256).
+        assert (N.lt (N_of_ascii c) 256).
+        clear H. induction c; repeat (match goal with
+                                      | B : bool |- _ => destruct B
+                                      end); simpl; unfold Nlt; eauto.
+        change (256%nat) with (N.to_nat 256).
+        apply Nomega.Nlt_out. eauto.
+        omega. change (pow2 8) with 256. omega.
+      }
+      subst. rewrite <- plus_n_O in H1. rewrite H1. clear H1.
+      rewrite Nnat.N2Nat.id. rewrite ascii_N_embedding. eauto.
     }
-    subst. rewrite <- plus_n_O in H1. rewrite H1. clear H1.
-    rewrite Nnat.N2Nat.id. rewrite ascii_N_embedding. eauto.
+    { intros env xenv xenv' n n' ext Eeq Penc.
+      destruct (decode_word n' xenv) as [ [ [? ? ] ? ] | ] eqn: ? ;
+        simpl in *; try discriminate.
+      injections.
+      eapply (proj2 Word_decode_correct) in Heqo; destruct_ex;
+        intuition; subst; eauto.
+      unfold encode_word_Spec in H0; computes_to_inv; injections.
+      repeat eexists; eauto.
+      repeat f_equal.
+      rewrite N_ascii_embedding.
+      rewrite NToWord_nat, wordToN_nat.
+      rewrite Nnat.Nat2N.id.
+      rewrite natToWord_wordToNat; eauto.
+      rewrite wordToN_nat.
+      pose proof (wordToNat_bound w).
+      simpl in H.
+      eapply Nomega.Nlt_in.
+      rewrite Nnat.Nat2N.id.
+      apply H.
+    }
   Qed.
 End Ascii.
