src/BinEncoders/Env/Lib2/FixListOpt.v
@@ -12,17 +12,29 @@ Section FixList.
   Context {transformer : Transformer B}.
 
   Variable A_predicate : A -> Prop.
-  Variable A_encode : A -> CacheEncode -> B * CacheEncode.
+  Variable A_encode_Spec : A -> CacheEncode -> Comp (B * CacheEncode).
+  Variable A_encode_Impl : A -> CacheEncode -> B * CacheEncode.
   Variable A_decode : B -> CacheDecode -> option (A * B * CacheDecode).
-  Variable A_decode_pf : encode_decode_correct_f cache transformer A_predicate A_encode A_decode.
+  Variable A_decode_pf : encode_decode_correct_f cache transformer A_predicate A_encode_Spec A_decode.
 
-  Fixpoint encode_list (xs : list A) (ce : CacheEncode) : B * CacheEncode :=
+  (* Ben: Should we do this with a FixComp instead? *)
+  Fixpoint encode_list_Spec (xs : list A) (ce : CacheEncode)
+    : Comp (B * CacheEncode) :=
+    match xs with
+    | nil => ret (transform_id, ce)
+    | x :: xs' => `(b1, env1) <- A_encode_Spec x ce;
+                    `(b2, env2) <- encode_list_Spec xs' env1;
+                    ret (transform b1 b2, env2)
+    end%comp.
+
+  Fixpoint encode_list_Impl (xs : list A) (ce : CacheEncode)
+    : B * CacheEncode :=
     match xs with
     | nil => (transform_id, ce)
-    | x :: xs' => let (b1, env1) := A_encode x ce in
-                  let (b2, env2) := encode_list xs' env1 in
-                      (transform b1 b2, env2)
-    end.
+    | x :: xs' =>  let (b1, env1) := A_encode_Impl x ce in
+                   let (b2, env2) := encode_list_Impl xs' env1 in
+                   (transform b1 b2, env2)
+    end%comp.
 
   Fixpoint decode_list (s : nat) (b : B) (cd : CacheDecode) : option (list A * B * CacheDecode) :=
     match s with
@@ -37,37 +49,55 @@ Section FixList.
       encode_decode_correct_f
         cache transformer
         (fun ls => |ls| = sz /\ forall x, In x ls -> A_predicate x)
-        encode_list (decode_list sz).
+        encode_list_Spec (decode_list sz).
   Proof.
-    unfold encode_decode_correct_f.
-    intros sz env env' xenv l l' ext Eeq Ppred Penc.
-    intuition; subst.
-    revert H0.
-    generalize dependent env. generalize dependent env'.
-    generalize dependent xenv.
-    generalize dependent l'. induction l.
-    { intros.
-      simpl in *; intuition; injections; simpl.
-      rewrite transform_id_left; eexists; eauto. }
-    { intros; simpl in *.
+    split.
+    {
+      intros env env' xenv l l' ext Eeq Ppred Penc.
       intuition; subst.
-      assert (A_predicate a) by eauto.
-      destruct (A_encode a env) eqn: ?.
-      destruct (encode_list l c) eqn: ?.
-      injections.
-      destruct (A_decode_pf _ _ _ _ _ (transform b0 ext) Eeq H Heqp) as [ ? [? ?] ].
-      destruct (IHl b0 xenv x c); intuition eauto.
-      rewrite <- transform_assoc.
-      eexists; intuition.
-      rewrite H1 by eauto; simpl; rewrite H4 by eauto; simpl.
-      eauto.
-      eauto.
+      revert H0.
+      generalize dependent env. generalize dependent env'.
+      generalize dependent xenv.
+      generalize dependent l'. induction l.
+      { intros.
+        simpl in *; intuition; computes_to_inv;
+          injections; simpl.
+        rewrite transform_id_left; eexists; eauto. }
+      { intros; simpl in *.
+        assert (A_predicate a) by eauto.
+        unfold Bind2 in Penc; computes_to_inv; subst.
+        destruct v; destruct v0; simpl in *.
+        injections.
+        destruct (proj1 A_decode_pf _ _ _ _ _ (transform b0 ext) Eeq H Penc) as [ ? [? ?] ].
+        setoid_rewrite <- transform_assoc; setoid_rewrite H1;
+          simpl.
+        destruct (IHl b0 xenv x c); intuition eauto.
+        setoid_rewrite H4; simpl.
+        eexists; intuition.
+      }
+    }
+    { induction sz; simpl; intros.
+      - injections; simpl; repeat eexists; intuition eauto.
+        symmetry; apply transform_id_left.
+      - destruct (A_decode bin env') as [ [ [? ?] ?] | ] eqn: ? ;
+          simpl in *; try discriminate.
+        destruct (decode_list sz b c) as [ [ [? ?] ?] | ] eqn: ? ;
+          simpl in *; try discriminate; injections.
+        eapply (proj2 A_decode_pf) in Heqo; eauto;
+          destruct_ex; intuition; subst.
+        eapply IHsz in Heqo0; eauto; destruct_ex; intuition; subst.
+        simpl.
+        eexists; eexists; intuition eauto.
+        computes_to_econstructor; eauto.
+        computes_to_econstructor; eauto.
+        rewrite transform_assoc; reflexivity.
+        subst; eauto.
     }
   Qed.
 
   Definition encode_list_body := (fun (acc: B * CacheEncode) x =>
-                                       let (bacc, env) := acc in
-                                       let (b1, env1) := A_encode x env in
+                                    let (bacc, env) := acc in
+                                       let (b1, env1) := A_encode_Impl x env in
                                        (transform bacc b1, env1)).
 
   Lemma encode_list_body_characterization :
@@ -78,7 +108,7 @@ Section FixList.
   Proof.
     induction xs; simpl.
     + intros; rewrite transform_id_right; reflexivity.
-    + intros; destruct (A_encode _ _).
+    + intros; destruct (A_encode_Impl _ _).
       rewrite IHxs, transform_id_left, (IHxs b).
       destruct (fold_left _ _ _).
       rewrite transform_assoc; reflexivity.
@@ -86,12 +116,12 @@ Section FixList.
 
   Lemma encode_list_as_foldl :
     forall xs env,
-      encode_list xs env =
+      encode_list_Impl xs env =
       fold_left encode_list_body xs (transform_id, env).
   Proof.
     induction xs; simpl.
     + reflexivity.
-    + intros; destruct (A_encode _ _).
+    + intros; destruct (A_encode_Impl _ _).
       rewrite IHxs, transform_id_left, (encode_list_body_characterization xs b c).
       destruct (fold_left _ _ _); reflexivity.
   Qed.
