src/BinEncoders/Env/Lib2/NatOpt.v
@@ -13,8 +13,12 @@ Section Nat.
   Context {transformer : Transformer B}.
   Context {transformerUnit : TransformerUnitOpt transformer bool}.
 
-  Definition encode_nat (n : nat) (ce : CacheEncode) : B * CacheEncode :=
-    encode_word (natToWord sz n) ce.
+  Definition encode_nat_Spec (n : nat) (ce : CacheEncode)
+    : Comp (B * CacheEncode) :=
+    encode_word_Spec (natToWord sz n) ce.
+
+  Definition encode_nat_Impl (n : nat) (ce : CacheEncode) : B * CacheEncode :=
+    encode_word_Impl (natToWord sz n) ce.
 
   Definition decode_nat (b : B) (cd : CacheDecode) : option (nat * B * CacheDecode) :=
     `(w, b, cd) <- decode_word (sz:=sz) b cd;
@@ -22,22 +26,34 @@ Section Nat.
 
   Local Open Scope nat.
   Theorem Nat_decode_correct :
-    encode_decode_correct_f cache transformer (fun n => n < pow2 sz) encode_nat decode_nat.
+    encode_decode_correct_f cache transformer (fun n => n < pow2 sz) encode_nat_Spec decode_nat.
   Proof.
-    unfold encode_decode_correct_f, encode_nat, decode_nat.
-    intros env xenv xenv' n n' ext Eeq Ppred Penc.
-    destruct (Word_decode_correct _ _ _ _ _ ext Eeq I Penc) as [? [? ?] ].
-    - rewrite H; simpl; eexists; intuition eauto.
-      repeat f_equal.
-      destruct (wordToNat_natToWord' sz n).
-      assert (x0 = 0).
-      { destruct x0; eauto.
-        rewrite <- H1 in Ppred. exfalso. simpl in Ppred.
-        clear - Ppred.
-        replace (wordToNat (natToWord sz n) + (pow2 sz + x0 * pow2 sz)) with
-        (pow2 sz + (wordToNat (natToWord sz n) + x0 * pow2 sz)) in Ppred by omega.
-        remember (wordToNat (natToWord sz n) + x0 * pow2 sz) as n'; clear Heqn'.
-        omega. }
-      rewrite H2 in H1. simpl in H1. rewrite <- plus_n_O in H1. eauto.
+    unfold encode_decode_correct_f, encode_nat_Spec, decode_nat.
+    split.
+    { intros env xenv xenv' n n' ext Eeq Ppred Penc.
+      destruct (proj1 Word_decode_correct _ _ _ _ _ ext Eeq I Penc) as [? [? ?] ].
+      - rewrite H; simpl; eexists; intuition eauto.
+        repeat f_equal.
+        destruct (wordToNat_natToWord' sz n).
+        assert (x0 = 0).
+        { destruct x0; eauto.
+          rewrite <- H1 in Ppred. exfalso. simpl in Ppred.
+          clear - Ppred.
+          replace (wordToNat (natToWord sz n) + (pow2 sz + x0 * pow2 sz)) with
+          (pow2 sz + (wordToNat (natToWord sz n) + x0 * pow2 sz)) in Ppred by omega.
+          remember (wordToNat (natToWord sz n) + x0 * pow2 sz) as n'; clear Heqn'.
+          omega. }
+        rewrite H2 in H1. simpl in H1. rewrite <- plus_n_O in H1. eauto.
+        }
+    { intros env xenv xenv' n n' ext Eeq Penc.
+      destruct (decode_word n' xenv) as [ [ [? ? ] ? ] | ] eqn: ? ;
+        simpl in *; try discriminate.
+      injections.
+      eapply (proj2 Word_decode_correct) in Heqo; destruct_ex;
+        intuition; subst; eauto.
+      unfold encode_word_Spec in H0; computes_to_inv; injections.
+      rewrite natToWord_wordToNat; repeat eexists; eauto.
+      apply wordToNat_bound.
+    }
   Qed.
 End Nat.
