src/BinEncoders/Env/Lib2/SumTypeOpt.v
@@ -16,11 +16,11 @@ Section SumType.
   Context {transformer : Transformer B}.
   Context {transformerUnit : TransformerUnitOpt transformer bool}.
 
-  Definition encode_SumType {m}
+  Definition encode_SumType_Spec {m}
              (types : Vector.t Type m)
-             (encoders : ilist (B := fun T => T -> CacheEncode -> B * CacheEncode) types)
+             (encoders : ilist (B := fun T => T -> CacheEncode -> Comp (B * CacheEncode)) types)
              (st : SumType types)
-    : CacheEncode -> B * CacheEncode :=
+    : CacheEncode -> Comp (B * CacheEncode) :=
     ith encoders (SumType_index types st) (SumType_proj types st).
 
   Definition decode_SumType {m}
@@ -44,7 +44,8 @@ Section SumType.
 
   Theorem SumType_decode_correct {m}
           (types : Vector.t Type m)
-          (encoders : ilist (B := fun T => T -> CacheEncode -> B * CacheEncode) types)
+          (encoders : ilist (B := fun T => T -> CacheEncode ->
+                                           Comp (B * CacheEncode)) types)
           (decoders : ilist (B := fun T => B -> CacheDecode -> option (T * B * CacheDecode)) types)
           (invariants : forall idx, Vector.nth types idx -> Prop)
           (encoders_decoders_correct : forall idx,
@@ -56,76 +57,34 @@ Section SumType.
           idx
     :
     encode_decode_correct_f cache transformer (fun st => SumType_index types st = idx /\ invariants _ (SumType_proj types st))
-                          (encode_SumType types encoders)
+                          (encode_SumType_Spec types encoders)
                           (decode_SumType types decoders idx).
   Proof.
-    revert types encoders decoders invariants encoders_decoders_correct.
-    unfold encode_decode_correct_f, encode_SumType, decode_SumType.
-    induction types.
-    - inversion idx.
-    - revert types IHtypes h; pattern n, idx; apply Fin.caseS;
-        clear n idx; intros; destruct H0.
-      + (* First element *)
-        destruct types.
-        * unfold SumType in data; simpl in *.
-          destruct (encoders_decoders_correct Fin.F1 _ _ _ _ _ ext H H2 H1) as [? [? ?] ]; simpl in *.
-          rewrite H3; simpl; eexists; eauto.
-        * destruct data; try discriminate; simpl in *.
-          destruct (encoders_decoders_correct Fin.F1 _ _ _ _ _ ext H H2 H1) as [? [? ?] ]; simpl in *.
-          match goal with
-            |- context [@prim_fst ?A ?B ?a ?z ?k] =>
-            replace (@prim_fst A B a z k) with (Some (h1, ext, x))
-              by (rewrite <- H3; reflexivity)
-          end.
-          simpl; eauto.
-      + (* Second element *)
-        destruct types; try discriminate.
-        destruct data; try discriminate.
-        assert (p = SumType_index (Vector.cons Type h0 n types) s) by
-            (apply Fin.FS_inj in H0;
-             rewrite <- H0; reflexivity).
-        assert (invariants
-                  (Fin.FS (SumType_index (Vector.cons Type h0 n types) s))
-                  (SumType_proj (Vector.cons Type h0 n types) s)) as H3' by
-            eapply H2.
-        assert (ith encoders
-                    (Fin.FS (SumType_index (Vector.cons Type h0 n types) s))
-                    (SumType_proj (Vector.cons Type h0 n types) s) env =
-                (bin, xenv)) as H1' by apply H1; clear H1.
-        assert (exists xenv' : CacheDecode,
-     (`(a, b', cd') <- ith (ilist_tl decoders) p (transform bin ext) env';
-      Some
-        (inj_SumType (Vector.cons Type h0 n types) p a, b',
-        cd')) = Some (s, ext, xenv') /\ Equiv xenv xenv').
-        { eapply (IHtypes p (ilist_tl encoders) (ilist_tl decoders)
-                 (fun idx => invariants (Fin.FS idx))); eauto.
-          intros.
-          destruct (encoders_decoders_correct (Fin.FS _) _ _ _ _ _ ext0 H1 H4 H5) as [? [? ?] ]; simpl in *.
-          eexists; intuition eauto.
-        }
+    split;
+      revert types encoders decoders invariants encoders_decoders_correct;
+      unfold encode_decode_correct_f, encode_SumType_Spec, decode_SumType.
+    { intros; intuition.
+      eapply (proj1 (encoders_decoders_correct _)) in H1; eauto;
         destruct_ex; intuition.
-        eexists; split; eauto.
-        match goal with
-            |- context [ith ?d ?idx ?tb ?env'] =>
-            destruct (ith d idx tb env') eqn: ?
-          end.
-        simpl in Heqo.
-        unfold ilist_tl in H4.
-        match type of H4 with
-          context [@ith ?A ?B ?m ?As ?il ?n ?il' ?M] =>
-          assert (@ith A B m As il n il' M = Some p0) as Heqo'
-              by (simpl; apply Heqo);
-            rewrite Heqo' in H4
-        end.
-        destruct p0 as [ [? ?] ?]; simpl in *.
-        injection H4; intros.
-        repeat f_equal; eauto.
-        match type of H4 with
-          context [@ith ?A ?B ?m ?As ?il ?n ?il' ?M] =>
-          assert (@ith A B m As il n il' M = None) as Heqo'
-              by (simpl; apply Heqo);
-            rewrite Heqo' in H4; discriminate
-        end.
+      subst; rewrite H1; simpl.
+      eexists; intuition eauto.
+      repeat f_equal.
+      rewrite inj_SumType_proj_inverse; reflexivity.
+    }
+    { intros.
+      destruct (ith decoders idx bin env') as [ [ [? ?] ? ] | ] eqn : ? ;
+        simpl in *; try discriminate; injections.
+      eapply (proj2 (encoders_decoders_correct idx)) in Heqo;
+        eauto; destruct_ex; intuition; subst.
+      exists x; exists x0; intuition;
+        try rewrite index_SumType_inj_inverse; eauto.
+      - pattern (SumType_index types (inj_SumType types idx n)),
+        (SumType_proj types (inj_SumType types idx n)).
+        eapply SumType_proj_inj; eauto.
+      - pattern (SumType_index types (inj_SumType types idx n)),
+        (SumType_proj types (inj_SumType types idx n)).
+        eapply SumType_proj_inj; eauto.
+    }
   Qed.
 End SumType.
 
