src/BinEncoders/Env/Lib2/WordOpt.v
@@ -22,8 +22,10 @@ Section Word.
     | WS b s' w' => transform_push_opt b (@encode_word' s' w')
     end.
 
-  Definition encode_word (w : word sz) (ce : CacheEncode) : B * CacheEncode :=
-    (encode_word' sz w, addE ce sz).
+  Definition encode_word_Impl (w : word sz) (ce : CacheEncode) : B * CacheEncode := (encode_word' sz w, addE ce sz).
+
+  Definition encode_word_Spec (w : word sz) (ce : CacheEncode) : Comp (B * CacheEncode) :=
+    ret (encode_word' sz w, addE ce sz).
 
   Fixpoint decode_word' (s : nat) (b : B) : option (word s * B) :=
     match s with
@@ -38,21 +40,50 @@ Section Word.
     Ifopt decode_word' sz b as decoded Then Some (decoded, addD cd sz) Else None.
 
   Theorem Word_decode_correct :
-    encode_decode_correct_f cache transformer (fun _ => True) encode_word decode_word.
+    encode_decode_correct_f cache transformer (fun _ => True) encode_word_Spec decode_word.
   Proof.
-    unfold encode_decode_correct, encode_word, decode_word.
-    intros env env' xenv w w' ext Eeq _ Penc.
-    inversion Penc; subst; clear Penc.
-    generalize dependent sz.
-    induction w; simpl in *.
-    { eexists; split; eauto; try rewrite !transform_id_left; 
-      eauto using add_correct. }
-    { rewrite transform_push_step_opt.
-      rewrite transform_push_pop_opt.
-      destruct_ex; intuition.
-      destruct (decode_word' n (transform (encode_word' n w) ext)) as [ [? ?] | ] eqn: ?; simpl in *; try discriminate.
-      injections; eexists; split; eauto using add_correct.
-      rewrite Heqo; simpl; f_equal.
-    }
+    unfold encode_decode_correct_f, encode_word_Spec, decode_word; split.
+    - intros env env' xenv w w' ext Eeq _ Penc.
+      computes_to_inv; injections.
+      generalize dependent sz.
+      induction w; simpl in *.
+      { eexists; split; eauto; try rewrite !transform_id_left;
+        eauto using add_correct. }
+      { rewrite transform_push_step_opt.
+        rewrite transform_push_pop_opt.
+        destruct_ex; intuition.
+        destruct (decode_word' n (transform (encode_word' n w) ext)) as [ [? ?] | ] eqn: ?; simpl in *; try discriminate.
+        injections; eexists; split; eauto using add_correct.
+        rewrite Heqo; simpl; f_equal.
+      }
+    - intros.
+      destruct (decode_word' sz bin)
+        as [ [? ?] | ] eqn: ?; simpl in *; try discriminate.
+      injections.
+      generalize dependent bin.
+      induction data; simpl in *.
+      { intros; computes_to_inv; intros; injection Heqo; clear Heqo;
+        intros; subst.
+        repeat eexists. eauto; try rewrite !transform_id_left;
+        eauto using add_correct.
+        apply add_correct; eauto.
+      }
+      { intros.
+        destruct (transform_pop_opt bin) as [ [? ?] | ] eqn: ? ;
+          simpl in *; try discriminate.
+        destruct (decode_word' n b1) as [ [? ? ] | ] eqn: ? ;
+          simpl in *; try discriminate.
+        injection Heqo; intros; subst.
+        apply Eqdep_dec.inj_pair2_eq_dec in H1; subst.
+        eapply IHdata in Heqo1.
+        destruct_ex; intuition; subst.
+        computes_to_inv; injections.
+        eexists; eexists; repeat split.
+        setoid_rewrite transform_push_step_opt.
+        eapply transform_pop_opt_inj; eauto.
+        rewrite transform_push_pop_opt; reflexivity.
+        apply add_correct; eauto.
+        eapply Peano_dec.eq_nat_dec.
+      }
   Qed.
 End Word.
