src/BinEncoders/Env/Common/ComposeOpt.v
@@ -10,8 +10,8 @@ Lemma compose_encode_correct A A' B
       (project : A -> A')
       (predicate : A -> Prop)
       (predicate' : A' -> Prop)
-      (encode1 : A' -> CacheEncode -> B * CacheEncode)
-      (encode2 : A -> CacheEncode -> B * CacheEncode)
+      (encode1 : A' -> CacheEncode -> Comp (B * CacheEncode))
+      (encode2 : A -> CacheEncode -> Comp (B * CacheEncode))
       (decode1 : B -> CacheDecode -> option (A' * B * CacheDecode))
       (decode1_pf : encode_decode_correct_f cache transformer predicate' encode1 decode1)
       (pred_pf : forall data, predicate data -> predicate' (project data))
@@ -21,20 +21,37 @@ Lemma compose_encode_correct A A' B
             (fun data => predicate data /\ project data = proj)
             encode2
             (decode2 proj))
-  : encode_decode_correct_f cache transformer predicate
-     (fun (data : A) (ctx : CacheEncode) =>
-      compose transformer (encode1 (project data)) (encode2 data) ctx)
+  : encode_decode_correct_f
+      cache transformer predicate
+      (fun (data : A) (ctx : CacheEncode) =>
+         `(bin, env') <- encode1 (project data) ctx;
+         `(bin', env'') <- encode2 data env';
+         ret (transform bin bin', env'')
+      )%comp
      (fun (bin : B) (env : CacheDecode) =>
         `(proj, rest, env') <- decode1 bin env;
           decode2 proj rest env').
 Proof.
-  intros env env' xenv data bin ext env_pm pred_pm com_pf.
-  unfold compose in com_pf.
-  destruct (encode1 (project data) env) as [b1 e1] eqn: eq1.
-  destruct (encode2 data e1) as [b2 e2] eqn: eq2.
-  injections.
-  destruct (decode1_pf _ _ _ _ _ (transform b2 ext) env_pm (pred_pf _ pred_pm) eq1) as [de [dp dt] ].
-  rewrite <- transform_assoc.
-  rewrite dp; simpl.
-  destruct (decode2_pf (project data) _ _ _ _ _ ext dt (conj pred_pm eq_refl) eq2); intuition eauto.
+  split.
+  { intros env env' xenv data bin ext env_pm pred_pm com_pf.
+    unfold Bind2 in com_pf; computes_to_inv; destruct v;
+      destruct v0.
+    destruct (proj1 decode1_pf _ _ _ _ _ (transform b0 ext) env_pm (pred_pf _ pred_pm) com_pf); intuition; simpl in *; injections.
+    setoid_rewrite <- transform_assoc; rewrite H0.
+    simpl.
+    destruct (proj1 (decode2_pf (project data)) _ _ _ _ _ ext H1 (conj pred_pm (eq_refl _)) com_pf'); intuition; simpl in *; injections.
+    rewrite H2; eauto. }
+  { intros.
+    destruct (decode1 bin env') as [ [ [? ?] ? ] | ] eqn : ? ; simpl in *;
+      try discriminate.
+    eapply (proj2 decode1_pf) in Heqo; eauto;
+      destruct_ex; intuition; subst.
+    eapply (proj2 (decode2_pf a)) in H0; eauto.
+    destruct_ex; intuition; subst.
+    eexists; eexists; repeat split.
+    repeat computes_to_econstructor; eauto.
+    simpl; rewrite transform_assoc; reflexivity.
+    eassumption.
+    simpl; eauto.
+  }
 Qed.
